WIP logical relation (almost get FTLR)

theories/logrel_ctx.v
@@ -61,6 +61,51 @@ Lemma safe_bind K e P Q :
 Proof.
   intros safeQ safeP.
   intros e' Hstep.
+  unfold safe_parametrized in safeQ.
+  (* inversion Hstep;subst. *)
+  (* - specialize (safeQ e). *)
+  (*   assert (e ~>* e) as Htrivial by econstructor. *)
+  (*   apply safeQ in Htrivial. *)
+  (*   destruct Htrivial as [(Hvale & HQ)| (e'' & Hstep')]. *)
+  (*   + apply safeP in HQ. *)
+  (*     unfold safe_parametrized in HQ. *)
+  (*     apply HQ in Hstep. *)
+  (*     destruct Hstep as [(Hvalv & HQv)| (e'' & Hstep')]. *)
+  (*     ++ left; firstorder. *)
+  (*     ++ right; exists e'';auto. *)
+  (*   + right. exists (fill K e''). by apply step_fill. *)
+  (* - fold (mstep b e') in H0. *)
+  (*   apply step_ectx in H as [Hv|(e'' & Hstep' & Hfill)]. *)
+  (*   + assert (e ~>* e) as Htrivial by econstructor. *)
+  (*     apply safeQ in Htrivial. *)
+  (*     destruct Htrivial as [(Hvale & HQ)| (e'' & Hstep')]. *)
+  (*     ++ apply safeP in HQ. *)
+  (*        unfold safe_parametrized in HQ. *)
+  (*        apply HQ in Hstep. *)
+  (*        destruct Hstep as [(Hvalv & HQv)| (e'' & Hstep')] *)
+  (*        ;[  left; firstorder | right; exists e'';auto]. *)
+  (*     ++ exfalso. *)
+  (*        by apply (is_val_stuck e e'') in Hv. *)
+  (*   + subst. *)
+  (*     assert (e ~>* e'') as Hstep2 by (econstructor;eauto). *)
+  (*     apply safeQ in Hstep2. *)
+  (*     destruct Hstep2 as [(Hvale'' & HQe'')| (e3 & Hstep3)]. *)
+  (*     ++ apply safeP in HQe''. *)
+  (*        unfold safe_parametrized in HQe''. *)
+  (*        apply HQe'' in H0. *)
+  (*        destruct H0 as [(Hvale' & HPe')| (e4 & Hstep4)]; firstorder. *)
+  (*     ++ *)
+  (*     assert (e ~>* e'') as Hstep4 by (econstructor;eauto). *)
+  (*     apply safeQ in Hstep4. *)
+  (*     destruct Hstep4 as [(Hvale'' & HQe'')| (e5 & Hstep5)]. *)
+  (*     +++ exfalso. by apply (is_val_stuck e'' e3) in Hvale''. *)
+  (*     +++ *)
+  (*       apply safeP in HQe''. *)
+  (*         unfold safe_parametrized in HQe''. *)
+  (*         apply HQe'' in H0. *)
+  (*         destruct H0 as [(Hvale' & HPe')| (e4 & Hstep4)]; firstorder. *)
+  (*       exfalso. *)
+  (*        by apply (is_val_stuck e e'') in Hv. *)
   apply mstep_ectx in Hstep as [(e'' & -> & Hstep)|(v & Hv & Hv1 & Hv2)].
   - apply safeQ in Hstep.
     destruct Hstep as [(Hv & HQv)|(e3 & He3)].
@@ -78,27 +123,32 @@ Qed.
 (* TODO Note that we are implicitly assuming that the domain of the partial mapping ξ in
 [∆ ⊢ τ ]ξ is always ∆ *)
 Fixpoint logrel_safe (Δ : tcontext) (ξ : substitution) (τ : ty) (v : expr) :=
-  is_val v /\
- match τ with
- | Ty_Var α => match (ξ !! α) with | None => True | Some P => P v end
- | Ty_Unit => v = <{ tt }>
- | Ty_Pair t1 t2 =>
-     exists e1 e2, is_val e1
-              /\ is_val e2
-              /\ v = <{ ⟨ e1, e2 ⟩ }>
-              /\ logrel_safe Δ ξ t1 e1
-              /\ logrel_safe Δ ξ t2 e2
- | Ty_Arrow t1 t2 =>
-     exists x e, v = <{ λ x, e }>
-            /\ (forall v', logrel_safe Δ ξ t1 v' -> safe_parametrized (logrel_safe Δ ξ t2) ( <{[ x / v'] e}>))
- | Ty_Forall α t =>
-     exists e, v = <{ Λ e }>
-            /\ forall (P: expr -> Prop), safe_parametrized (logrel_safe ({[α]}∪ Δ) (<[α := P]> ξ) t) e
- end.
+  dom ξ = Δ /\
+    is_val v /\
+    match τ with
+    | Ty_Var α => match (ξ !! α) with | None => False | Some P => P v end
+    | Ty_Unit => v = <{ tt }>
+    | Ty_Pair t1 t2 =>
+        exists e1 e2, is_val e1
+                 /\ is_val e2
+                 /\ v = <{ ⟨ e1, e2 ⟩ }>
+                 /\ logrel_safe Δ ξ t1 e1
+                 /\ logrel_safe Δ ξ t2 e2
+    | Ty_Arrow t1 t2 =>
+        exists x e, v = <{ λ x, e }>
+               /\ (forall v', logrel_safe Δ ξ t1 v' -> safe_parametrized (logrel_safe Δ ξ t2) ( <{[ x / v'] e}>))
+    | Ty_Forall α t =>
+        exists e, v = <{ Λ e }>
+             /\ forall (P: expr -> Prop), safe_parametrized (logrel_safe ({[α]}∪ Δ) (<[α := P]> ξ) t) e
+end.
 
 Lemma safe_is_val Δ ξ v τ : logrel_safe Δ ξ τ v -> is_val v.
 Proof.
-  induction τ; simpl ; intros; destruct H;auto.
+  induction τ; simpl ; intros; destruct H as (?&?&?);auto.
+Qed.
+
+Lemma safe_domain  Δ ξ v τ : logrel_safe Δ ξ τ v -> dom ξ = Δ.
+  induction τ; simpl ; intros; destruct H as (?&?&?);auto.
 Qed.
 
 Lemma logrel_subst Δ ξ τ τ' v α :
@@ -112,7 +162,8 @@ Proof.
     generalize dependent ξ.
     generalize dependent Δ.
     induction τ; intros * Hsafe; simpl in *; auto.
-  + split; [by apply safe_is_val in Hsafe|].
+  + split; [apply safe_domain in Hsafe; set_solver|].
+    split; [by apply safe_is_val in Hsafe|].
     destruct (α =? s)%string eqn:Heq.
     * apply String.eqb_eq in Heq; subst.
       assert (Heq: <[s:=logrel_safe Δ ξ τ']> ξ !! s = Some (logrel_safe Δ ξ τ'))
@@ -124,33 +175,36 @@ Proof.
       by (apply lookup_insert_ne;auto).
       rewrite Hmap.
       apply Hsafe.
+  + destruct Hsafe as (<- & Hval & ->).
+    firstorder set_solver.
   + (* pair *)
-    destruct Hsafe as (Hval & v1 & v2 & Hval1 & Hval2 & -> & Hsafe1 & Hsafe2).
-    split;auto.
+    destruct Hsafe as (Hdom & Hval & v1 & v2 & Hval1 & Hval2 & -> & Hsafe1 & Hsafe2).
+    split;auto;[set_solver|split;auto].
     exists v1, v2.
     repeat(split;auto).
   + (* lambda *)
-    destruct Hsafe as (Hval & x & e & -> & Hsafe).
-    split;auto.
+    destruct Hsafe as (Hdom & Hval & x & e & -> & Hsafe).
+    split;auto;[set_solver|split;auto].
     exists x, e.
     split;auto.
     set ( ξ' := (<[α:=logrel_safe Δ ξ τ']> ξ) ).
+    set ( Δ' := ({[α]} ∪ Δ)).
     intros.
     intros e' Hstep.
     admit.
   + (* poly *)
     destruct (α =? s)%string eqn:Heq ; simpl in Hsafe
-    ;destruct Hsafe as (Hval & e & Hv & Hsafe); split;auto; exists e
-    ; split; auto
-    ; intros;
-      specialize (Hsafe P).
-    replace ( {[s]} ∪ ({[α]} ∪ Δ)) with ({[α]} ∪ ({[s]} ∪ Δ)) by set_solver.
+    ;destruct Hsafe as (Hdom & Hval & e & Hv & Hsafe);
+      split ; try set_solver;split;auto
+    ; exists e ; split; auto ; intros; specialize (Hsafe P)
+    ; replace ( {[s]} ∪ ({[α]} ∪ Δ)) with ({[α]} ∪ ({[s]} ∪ Δ)) by set_solver.
     intros e' Hstep.
     apply Hsafe in Hstep.
     destruct Hstep; [left|right].
-    (* I need to be able to swap α and s *)
+    destruct H as [Hvale' Hlogrel].
+    split;auto.
     admit.
-    admit.
+    auto.
     admit.
   - admit.
 Admitted.
@@ -160,19 +214,25 @@ Lemma logrel_weaken Δ ξ τ v α P :
   ((logrel_safe Δ ξ τ v) <->
   (logrel_safe Δ  (<[α := P]> ξ) τ v)).
 Proof.
-
   split; intros Hsafe;
   generalize dependent v;
   induction τ; intros; simpl in *;
-  destruct Hsafe; split; auto.
-  - unfold not in H.
+  destruct Hsafe as (Hdom & Hval & Hsafe).
+  - (* Var *)
+    split; [|split]; auto.
+    destruct (decide (α = s)%string); subst.
+    exfalso; apply H; apply free_var.
+    admit.
+    unfold not in H.
     destruct (decide (α = s)%string); subst.
     + (* \alpha = s --> contradiction with free *)
       exfalso; apply H; apply free_var.
     + replace (<[α:=P]> ξ !! s) with (ξ !! s)
     by (symmetry ; apply lookup_insert_ne;auto).
     auto.
-  - destruct H1 as (v1 & v2 & Hv1 & Hv2 & Hv& Hsafe1 & Hsafe2).
+  - split;[admit|];auto.
+  - split;[admit|split];auto.
+    destruct Hsafe as (v1 & v2 & Hv1 & Hv2 & Hv& Hsafe1 & Hsafe2).
     exists v1, v2.
     repeat(split;auto).
     apply IHτ1;auto; intro; apply H; by apply free_pair1.
@@ -228,15 +288,11 @@ Definition context_var Γ : list string :=
   map (fun x => match x with (x1,x2) => x1 end) (gmap_to_list Γ).
   (* (gmap_to_list Γ).*1 . *)
 
-Lemma subst_term_seq_insert Γ vs x τ v e :
+Lemma subst_term_seq_insert e :
+  forall Γ vs x τ v,
   (subst_term_seq (context_var (<[x:=τ]> Γ)) (v :: vs) e) =
     subst_term x v (subst_term_seq (context_var Γ) (vs) e).
 Proof.
-  generalize dependent Γ.
-  generalize dependent vs.
-  generalize dependent x.
-  generalize dependent τ.
-  generalize dependent v.
   induction e; intros ; auto; cbn.
   - (* var *)
     induction Γ using map_ind.
@@ -269,7 +325,37 @@ Proof.
     by rewrite IHe.
 Admitted.
 
-Theorem fundamental_theorem Δ Γ τ e :
+Lemma logrel_safe_list_dom: forall Δ Γ ξ vs,
+  logrel_seq Δ Γ ξ vs -> dom ξ = Δ.
+Admitted.
+
+Lemma step_fst v1 v2:
+  is_val v1 ->
+  is_val v2 ->
+  <{ fst (⟨ v1, v2 ⟩) }> ~> v1.
+Proof.
+  intros; eapply (Step _ _ EmptyCtx); eauto.
+Qed.
+
+Lemma step_snd v1 v2:
+  is_val v1 ->
+  is_val v2 ->
+  <{ snd (⟨ v1, v2 ⟩) }> ~> v2.
+Proof.
+  intros; eapply (Step _ _ EmptyCtx); eauto.
+Qed.
+
+Lemma step_app x e v:
+  is_val v ->
+  <{ (λ x, e) v }> ~>  <{ [x / v]e }>.
+Proof.
+  intros; eapply (Step _ _ EmptyCtx); eauto.
+Qed.
+
+Hint Resolve step_fst step_snd step_app : core.
+
+Theorem fundamental_theorem :
+  forall Δ Γ τ e ,
   Δ;Γ ⊢ e ∈ τ -> (forall ξ vs, logrel_seq Δ Γ ξ vs
                          -> safe_parametrized
                            (logrel_safe Δ ξ τ) (subst_term_seq (context_var Γ) vs e)).
@@ -278,68 +364,140 @@ Proof.
   - (* T_Unit *)
     apply safe_val; auto.
     simpl in * ; split ; auto.
+    by eapply logrel_safe_list_dom.
   - (* T_Var *)
     induction Γ using map_ind.
-    unfold replace_var.
+    exfalso. (* from H, error *) admit.
     (* TODO from H, we know that x \in (context_var \Gamma), and thus we can replace
        the variable *)
     admit.
-    admit.
   - (* T_Prod *)
-    (* TODO how to cbn just subst_term_seq ? *)
-    (* eapply (safe_bind (LPairCtx EmptyCtx _ )); econstructor; eauto. *)
-    (* 2:{ cbn in *. inversion H3; cbn.  } *)
-    cbn.
-    repeat intro.
     pose proof H1 as H1'.
     apply IHtyping_judgment1 in H1.
     apply IHtyping_judgment2 in H1'.
-    unfold safe_parametrized in H1,H1'.
-    admit.
+    simpl subst_term_seq.
+    set (e1' := (subst_term_seq (context_var Γ) vs e1) ) in *.
+    set (e2' := (subst_term_seq (context_var Γ) vs e2) ) in *.
+    replace (expr_pair e1' e2') with (fill (LPairCtx EmptyCtx e2') e1') by auto.
+    eapply safe_bind;eauto.
+    intros ve1 Hsafe_ve1.
+    simpl fill.
+    assert (is_val ve1) by (by eapply safe_is_val).
+    apply is_val_inversion in H2. destruct H2 as [v1 ->].
+    replace (expr_pair (of_val v1) e2') with (fill (RPairCtx EmptyCtx v1) e2')
+    by auto.
+    eapply safe_bind;eauto.
+    intros ve2 Hsafe_ve2.
+    assert (is_val ve2) by (by eapply safe_is_val).
+    apply is_val_inversion in H2. destruct H2 as [v2 ->].
+    simpl fill.
+    intros e' He'.
+    assert (Hval_pair: (is_val (expr_pair (of_val v1) (of_val v2)))) by
+    (constructor; apply is_val_of_val).
+    apply is_val_step in He'; auto;subst.
+    left. split; auto.
+    simpl.
+    split;[by eapply safe_domain; eassumption|split;auto].
+    exists (of_val v1). exists (of_val v2).
+    repeat (split;auto using is_val_of_val).
   - (* T_Fst *)
-
     cbn.
-    (* apply IHtyping_judgment in H0. *)
-    (* destruct H0 as (is_val_e & e1 & e2 & is_val_e1 & is_val_e2 & v_pair *)
-    (*                 & Hsafe_e1 & Hsafe_e2). *)
-    (* rewrite v_pair. *)
-    (* backward logrel_safe, because fst(e1,e2) -> e1, it suffices to show on e1 *)
-    admit.
+    apply IHtyping_judgment in H0.
+    replace (expr_fst (subst_term_seq (context_var Γ) vs e))
+              with (fill (FstCtx EmptyCtx) (subst_term_seq (context_var Γ) vs e)) by auto.
+    eapply safe_bind;eauto .
+    intros v Hrel.
+    cbn in Hrel.
+    destruct Hrel as (Hdom & Hval & v1 & v2 & Hv1 & Hv2 & -> & Hrel1 & Hrel2).
+    cbn.
+    eapply safe_step with (e' := v1);auto.
+    repeat intro.
+    apply is_val_step in H1;subst;auto.
   - (* T_Snd *)
     cbn.
-    (* rewrite subst_term_seq_snd; cbn in *. *)
-    (* apply IHtyping_judgment in H0. *)
-    (* destruct H0 as (is_val_e & e1 & e2 & is_val_e1 & is_val_e2 & v_pair *)
-    (*                 & Hsafe_e1 & Hsafe_e2). *)
-    (* rewrite v_pair. *)
-    admit.
-  - (* T_Lam *)
+    apply IHtyping_judgment in H0.
+    replace (expr_snd (subst_term_seq (context_var Γ) vs e))
+              with (fill (SndCtx EmptyCtx) (subst_term_seq (context_var Γ) vs e)) by auto.
+    eapply safe_bind;eauto .
+    intros v Hrel.
+    cbn in Hrel.
+    destruct Hrel as (Hdom & Hval & v1 & v2 & Hv1 & Hv2 & -> & Hrel1 & Hrel2).
     cbn.
-    set( v :=
-           match find (String.eqb x) (context_var Γ) with
-           | Some _ => <{ λ x, e }>
-           | None => (expr_abs x (subst_term_seq (context_var Γ) vs e))
-           end
-       ).
-    assert (is_val v).
-    { destruct (find (String.eqb x) (context_var Γ)) ; subst v; auto. }
-    apply safe_val;auto.
-    split;auto.
-    exists x. exists (subst_term_seq (context_var Γ) vs e).
-    split.
-    + subst v. admit.
-    + intros.
-      assert ( logrel_seq Δ (<[x := τ1]> Γ) ξ (v'::vs)). admit.
-    (* apply IHtyping_judgment in H2. simpl in H2. *)
-    (* cbn in H2. *)
-    (* unfold subst_term_seq in H2. *)
-    (* rewrite subst_term_seq_insert in H2. *)
-    (* apply H2. *)
+    eapply safe_step with (e' := v2);auto.
+    repeat intro.
+    apply is_val_step in H1;subst;auto.
+  - (* T_Lam *)
+    apply safe_val.
+    { simpl.
+      destruct (find (String.eqb x) (context_var Γ)); constructor. }
+    split; eauto using logrel_safe_list_dom.
+    split;[simpl;destruct (find (String.eqb x) (context_var Γ)); constructor|].
+    destruct (find (String.eqb x) (context_var Γ)) eqn:Heq.
+    + simpl. rewrite Heq.
+      eexists;eexists;split;eauto.
+      intros.
+      assert (logrel_seq Δ (<[x:= τ1]>Γ) ξ (v'::vs)).
+      { unfold logrel_seq.
+        admit.
+      }
+      apply IHtyping_judgment in H2. admit.
+    + simpl. rewrite Heq.
+      eexists;eexists;split;eauto.
+      intros.
+      assert (logrel_seq Δ (<[x:= τ1]>Γ) ξ (v'::vs)).
+      { unfold logrel_seq.
+        admit.
+      }
+      apply IHtyping_judgment in H2.
       admit.
   - (* T_App *)
-    admit.
+    simpl subst_term_seq.
+    pose proof H1 as H1'.
+    apply IHtyping_judgment1 in H1.
+    apply IHtyping_judgment2 in H1'.
+    set (fs := (subst_term_seq (context_var Γ) vs e)) in *.
+    set (arg := (subst_term_seq (context_var Γ) vs e')) in *.
+    replace (expr_app fs arg)
+              with (fill (LAppCtx EmptyCtx arg) fs) by auto.
+    eapply safe_bind;eauto .
+    intros fv Hfv.
+    simpl fill.
+    assert (is_val fv) by (by eapply safe_is_val).
+    apply is_val_inversion in H2. destruct H2 as [f ->].
+    replace (expr_app (of_val f) arg) with (fill (RAppCtx EmptyCtx f) arg)
+    by auto.
+    eapply safe_bind;eauto.
+    intros argv Hargv.
+    simpl fill.
+    assert (is_val argv) by (by eapply safe_is_val).
+    apply is_val_inversion in H2. destruct H2 as [v ->].
+    destruct Hfv as (Hdom & Hvalf & x & fe & -> & Hsafe_app).
+    eapply safe_step with (e' := subst_term x (of_val v) fe).
+    eapply (Step _ _ EmptyCtx); eauto; econstructor. apply is_val_of_val.
+    by apply Hsafe_app.
   - (* T_TLam *)
-    admit.
+    simpl subst_term_seq.
+    apply safe_val; [constructor|cbn].
+    split; eauto using logrel_safe_list_dom.
+    split;[constructor|].
+    eexists;split;[reflexivity|].
+    intros.
+    apply IHtyping_judgment.
+    apply logrel_seq_weaken;auto.
   - (* T_TApp *)
-    admit.
+    simpl subst_term_seq.
+    apply IHtyping_judgment in H0.
+    set (es := (subst_term_seq (context_var Γ) vs e)) in *.
+    replace (expr_tapp es)
+              with (fill (TAppCtx EmptyCtx) es) by auto.
+    eapply safe_bind ;eauto.
+    intros ev Hev.
+    simpl fill.
+    destruct Hev as (Hdom & Hvalv & f & -> & Hsafe_app).
+    eapply safe_step with (e' := f).
+    eapply (Step _ _ EmptyCtx); eauto; econstructor.
+    specialize (Hsafe_app (logrel_safe Δ ξ τ')).
+    eapply safe_mono.
+    2: apply Hsafe_app.
+    intros; by apply logrel_subst.
 Admitted.
